src/SepLogic/Mem/Upd.v
@@ -14,6 +14,9 @@ Section Upd.
   Definition upd m a v : mem A V :=
     fun a' => if a == a' then Some v else m a'.
 
+  Definition delete m a : mem A V :=
+    fun a' => if a == a' then None else m a'.
+
   Theorem upd_eq : forall m a v,
       upd m a v a = Some v.
   Proof.
@@ -37,8 +40,25 @@ Section Upd.
     destruct matches.
   Qed.
 
+  Theorem delete_eq : forall m a,
+      delete m a a = None.
+  Proof.
+    unfold delete; intros.
+    destruct matches.
+  Qed.
+
+  Theorem delete_neq : forall m a a',
+      a <> a' ->
+      delete m a a' = m a'.
+  Proof.
+    unfold delete; intros.
+    destruct matches.
+  Qed.
+
 End Upd.
 
 Hint Rewrite upd_eq : upd.
+Hint Rewrite delete_eq : upd.
 Hint Rewrite upd_upd : upd.
 Hint Rewrite upd_neq using (solve [ auto || congruence ]) : upd.
+Hint Rewrite delete_neq using (solve [ auto || congruence ]) : upd.
